DafnyVerification/kShortesPathVertices.dfy
@@ -1,3 +1,4 @@
+
 class PriorityQueue<T>
 {
 	var val: seq<T>;
@@ -38,29 +39,17 @@ class PriorityQueue<T>
 
 class Vertex
 {
-	var name: string;
+	var name: int;
 	var numShortestPath: nat;
-}
 
-class Path
-{
-	var flights: seq<Flight>;
-
-	constructor(newFlights:seq<Flight>)
-	ensures flights == newFlights;
-	modifies this;
+	function method equals(v1: Vertex) :bool
+	requires v1 != null;
+	reads *;
 	{
-		var i := 0;
-		flights := [];
-		while i < |newFlights|
-		invariant i <= |newFlights|;
-		{
-			flights := flights + [newFlights[i]];
-			i := i + 1;
-		}
+		v1.name == this.name
 	}
-	
 }
+
 
 class Flight
 {
@@ -68,7 +57,8 @@ class Flight
 	var destination: Vertex;
 	var cost: int;
 
-	constructor(o: Vertex, d: Vertex, c: int)
+	constructor Init(o: Vertex, d: Vertex, c: int)
+	requires o != null && d !=null;
 	requires cost >= 0;
 	modifies this;
 	{
@@ -78,58 +68,96 @@ class Flight
 	}
 }
 
-class FlightPlan
-{
-	var list: seq<Path>;
-
-	constructor ()
-	modifies this;
-	ensures list == []
-	{
-		list := [];
-	}
-}
-
 class Graph
 { 
 	var vertices : set<Vertex> ; 
-	var edges: map<Vertex,seq<Vertex>>; 
+	ghost var edgesMap: map<Vertex, set<Vertex>>;
+	var edges: seq<Flight>;
 
-	method getNeighbours(f: Flight) returns (n:seq<Vertex>)
-	requires f.destination in vertices; 
+
+	/*predicate noNull()
+	reads *;
 	{
-		n := edges[f.destination];
+		(forall u:Vertex :: u in vertices ==> u != null) &&
+		(forall p:Flight :: p in edges ==> p != null && p.origin != null && p.destination != null)
+	}*/
+
+	method getNeighbours(f: Flight) returns (n:seq<Flight>)
+	//requires noNull();
+	requires f != null && f.destination != null && f.origin != null;
+	requires f.destination in vertices;
+	requires f in edges;
+	requires forall p:Flight :: p in edges && p != null
+	//ensures forall p:Flight :: p in n ==> f.destination == p.origin;
+	{
+		var i := 0;
+		n := [];
+		while i < |edges|
+		invariant i <= |edges|
+		invariant forall j:nat :: j < i ==> edges[j] != null;
+		{
+			if f.destination == edges[i].origin
+			{
+				n := n + [edges[i]];
+			}
+
+			i := i + 1;
+		}
 	}
 
-} 
+	method getNeighboursVertex(v: Vertex) returns (n:seq<Flight>)
+	//requires noNull();
+	requires v != null;
+	requires v in vertices;
+	requires v in edgesMap;
+	requires forall p:Flight :: (p in edges) ==> p != null;
+	//ensures forall p:Flight :: p in n ==> v == p.origin;
+	{
+		var i := 0;
+		n := [];
+		while i < |edges|
+		invariant i <= |edges|
+		//invariant forall j:nat :: j < i ==> n[j] != null && n[j].origin != null;
+		decreases |edges| - i;
+		{
+			if v == edges[i].origin
+			{
+				n := n + [edges[i]];
+			}
 
+			i := i + 1;
+		}
+	}
+
+}
 
 predicate well_formed(g:Graph) 
-reads g; 
+reads *; 
 { 
 	g != null && 
 	null !in g.vertices && 
 	// here u in g.edges says that u is in the domain of the map g.edges
-	(forall u:Vertex :: ( (u in g.edges)  ==> u in g.vertices )) && 
-	(forall u:Vertex :: ( u in g.vertices  ==> u in g.edges )) && 
-	forall u:Vertex :: u in g.edges  ==> forall v:Vertex ::  v in g.edges[u] ==> (v != null && v in g.vertices)   
+	(forall u:Vertex :: ( (u in g.edgesMap)  ==> u in g.vertices )) && 
+	(forall u:Vertex :: ( u in g.vertices  ==> u in g.edgesMap )) && 
+	(forall u:Vertex :: u in g.edgesMap  ==> forall v:Vertex ::  v in g.edgesMap[u] ==> (v != null && v in g.vertices) )&&
+	 forall f:Flight :: f in g.edges ==> (f != null && f.origin != null && f.destination != null)
 }
 
 
 
 predicate path(from:Vertex,to:Vertex, p:seq<Vertex>,g:Graph) 
-reads p,g; 
+reads *; 
 {  
 	well_formed(g) && from in g.vertices && to in g.vertices && 
 	|p| > 0 && 
 	(forall v:Vertex :: v in p ==> v in g.vertices)  && 
-	from == p[0] && to == p[|p|-1] && forall n:nat :: (n<|p|-1 ==> p[n+1] in g.edges[p[n]]) 
+	from == p[0] && to == p[|p|-1] && forall n:nat :: (n<|p|-1 ==> p[n+1] in g.edgesMap[p[n]]) 
 }
 
 lemma path_extend(from:Vertex,to:Vertex,next:Vertex,p:seq<Vertex>,g:Graph)
 requires well_formed(g) && from in g.vertices && to in g.vertices && next in g.vertices ; 
 requires path(from,to,p,g); 
-requires next in g.edges[to] ; 
+requires next in g.edgesMap[to] ; 
 ensures path(from,next,p+[next],g); 
 {
 // Dafny knows this already 
@@ -138,8 +166,8 @@ ensures path(from,next,p+[next],g);
 
 
 
-method search(from:Vertex, to:Vertex, g:Graph, k: int) returns (P: set<Path>) 
-requires from in g.vertices && to in g.vertices && well_formed(g); 
+method search(from:Vertex, to:Vertex, g:Graph, k: int) returns (P: set<seq<Flight>>) 
+requires well_formed(g) && from in g.vertices && to in g.vertices; 
 requires k > 0;
 modifies set v:Vertex | v in g.vertices; 
 ensures |P| <= k; //where P is a set of k Paths and a Path is a set of Edges
@@ -150,9 +178,23 @@ decreases * ; // This is needed here to allow decreases * on the loop
 
 	//var P :seq<FlightPlan>; //Set of shortest paths
 	P := {};
-	var B := new PriorityQueue<FlightPlan>.Init(); //Heap data structure containing paths 
+	var q := new PriorityQueue<seq<Flight>>.Init(); //Heap data structure containing paths 
 	forall u:Vertex | u in g.vertices { u.numShortestPath := 0; }
-	B.offer(from.path);
+	
+	var i := 0;
+	assert from in g.vertices;
+	assert forall p:Flight :: p in g.edges ==> p != null && p.origin != null && p.destination != null;
+	var neighbours := g.getNeighboursVertex(from);
+	while i < |neighbours|
+	{
+		//var path := new Path.Init();
+		//path.addFlight(neighbours[i]);
+		var path := [neighbours[i]];
+		q.offer(path);
+		i := i + 1;
+	}
+	/*
+	//q.offer(from.getPaths);
 
 	while !B.isEmpty() && to.numShortestPath < k
 	decreases *;//(k - to.numShortestPath), B//ignore termination for now
@@ -174,20 +216,17 @@ decreases * ; // This is needed here to allow decreases * on the loop
 		
 		if(u.numShortestPath <= k)
 		{
-			/*forall v:Vertex | v in u.adjacent 
-			{
-				P_v = P_u + [v];
-				B.offer(P_v);
-			}*/
+
 			var i := 0;
 			while i < |u.adjacent|
 			decreases |u.adjacent| - i; 
 			{
 				var v := u.adjacent[i];
-				var adj := new Edge.Init(u.getFlights());
+				var adj := new Path.Init(u.getFlights());
 				i := i + 1;
 			}
 		}
-	}
-}
 
+	}
+*/
+}
